isabelle_code/Automata/implementation/RBT_NFAImpl.thy
@@ -8,9 +8,11 @@ imports  "Collections.Collections"
           DFAByLTS 
 begin
 
-
 interpretation rs_nfa_defs: nfa_dfa_by_lts_interval_defs rs_ops rs_ops
                             rs_ops rs_ops rs_lts_ops rs_lts_ops
+
+interpretation rs_nfa_defs: nfa_dfa_by_lts_interval_defs rs_ops
+                            rs_ops rs_ops rs_ops rs_lts_ops rs_lts_ops
   by intro_locales
 
 thm rs.correct
